\subsection{Inertia Tensor:}
$\begin{bmatrix}\label{ma:Inertia Tensor}
  A & -H & -G \\
  -H & B & -F \\
  -G & -F & C
\end{bmatrix}$

\begin{equation}\label{eq:Moments of Inertia}
A=\sum\rho\left({x}_{2}^{2}+{x}_{3}^{2}\right)
\qquad
B=\sum\rho\left({x}_{1}^{2}+{x}_{3}^{2}\right)
\qquad
C=\sum\rho\left({x}_{1}^{2}+{x}_{2}^{2}\right)
\end{equation}
\begin{equation}\label{eq:Product of Inertia}
F=\sum\rho\left({x}_{2}{x}_{3}\right)
\qquad
G=\sum\rho\left({x}_{1}+{x}_{3}\right)
\qquad
H=\sum\rho\left({x}_{1}+{x}_{2}\right)
\end{equation}